@base <http://ns.ontowiki.net/SysOnt/Site/>.
@prefix rdf: <http://www.w3.org/1999/02/22-rdf-syntax-ns#>.
@prefix rdfs: <http://www.w3.org/2000/01/rdf-schema#>.
@prefix owl: <http://www.w3.org/2002/07/owl#>.
@prefix site: <http://ns.ontowiki.net/SysOnt/Site/>.
@prefix skos: <http://www.w3.org/2004/02/skos/core#>.
@prefix xsd: <http://www.w3.org/2001/XMLSchema#>.
@prefix foaf: <http://xmlns.com/foaf/0.1/>.
@prefix doap: <http://usefulinc.com/ns/doap#>.
@prefix vann: <http://purl.org/vocab/vann/>.
@prefix schema: <http://schema.org/>.

###
# Classes
###

site:Navigation a rdfs:Class ;
  rdfs:comment "an RDF sequence resource which is used by the site extensions menu helper" ;
  rdfs:label "Navigation" ;
  rdfs:subClassOf rdf:Seq ;
  schema:isSimilarTo schema:SiteNavigationElement;
  skos:note "menu items can have a special label with site:menuLabel" ;
  rdfs:isDefinedBy <http://ns.ontowiki.net/SysOnt/Site/> .

site:MovedResource a owl:Class;
  rdfs:comment "a resource which is moved to another namespace or which URI is changed for some reason." ;
  skos:note "moved resources should link with site:seeAlso to the new URI" ;
  rdfs:label "Moved Resource";
  rdfs:isDefinedBy <http://ns.ontowiki.net/SysOnt/Site/> .

site:DeletedResource a owl:Class;
  rdfs:comment "a resource which was deleted for some reason." ;
  skos:note "deleted resources should link with site:seeAlso to more generic resources or similar resources" ;
  rdfs:label "Deleted Resource";
  rdfs:isDefinedBy <http://ns.ontowiki.net/SysOnt/Site/> .

site:SiteMap a owl:Class;
  rdfs:comment "a XML resource according to sitemap.org" ;
  rdfs:label "Sitemap";
  rdfs:isDefinedBy <http://ns.ontowiki.net/SysOnt/Site/> .

site:TemplateOption a owl:Class;
  rdfs:subClassOf rdf:Property;
  rdfs:comment "the class of site specific template relevant options which can be used on resources, classes and datasets";
  rdfs:label "Template Option";
  rdfs:isDefinedBy <http://ns.ontowiki.net/SysOnt/Site/> .

###
# Properties
###

site:seeAlso a owl:ObjectProperty, owl:FunctionalProperty;
  rdfs:comment "If a requested resources links with this property to another resource, the server should forward to this resource";
  rdfs:subPropertyOf rdfs:seeAlso;
  rdfs:label "seeAlso (site)";
  rdfs:isDefinedBy <http://ns.ontowiki.net/SysOnt/Site/> .

site:menuLabel a owl:DatatypeProperty, owl:FunctionalProperty ;
  rdfs:comment "if present, the navigation list helper uses this literal for the display name of the menu item" ;
  rdfs:label "menu label" ;
  rdfs:subPropertyOf skos:altLabel ;
  rdfs:isDefinedBy <http://ns.ontowiki.net/SysOnt/Site/> .

site:content a owl:DatatypeProperty ;
  rdfs:comment "the main content of a resource in an encoded text of a specific encoding datatype, e.g. sysont:Markdown." ;
  rdfs:label "main content" ;
  rdfs:subPropertyOf <http://purl.org/rss/1.0/modules/content/encoded> ;
  rdfs:isDefinedBy <http://ns.ontowiki.net/SysOnt/Site/> .

site:templateOption a owl:DatatypeProperty ;
  rdfs:comment "this property is used to forward specific options to the rendering templates" ;
  rdfs:label "template option" ;
  rdfs:isDefinedBy <http://ns.ontowiki.net/SysOnt/Site/> .

site:abbrevation a owl:DatatypeProperty ;
  rdfs:comment "the abbrevation of a resource is used e.g. as a url naming part as well as can be used for better searching." ;
  rdfs:label "abbrevation" ;
  rdfs:subPropertyOf skos:altLabel ;
  rdfs:isDefinedBy <http://ns.ontowiki.net/SysOnt/Site/> .

site:classTemplate a owl:DatatypeProperty, owl:FunctionalProperty ;
  rdfs:comment "identifies the template which is used to render the HTML representations of the resources of a class" ;
  rdfs:domain owl:Class ;
  rdfs:label "class template" ;
  rdfs:range xsd:string ;
  rdfs:isDefinedBy <http://ns.ontowiki.net/SysOnt/Site/> .

site:template a owl:DatatypeProperty, owl:FunctionalProperty ;
  rdfs:comment "identifies the template which is used to render the HTML representation of a specific resources";
  skos:note "this attribute overwrites the site:classTemplate property" ;
  rdfs:label "template" ;
  rdfs:range xsd:string ;
  rdfs:isDefinedBy <http://ns.ontowiki.net/SysOnt/Site/> .

###
# Vocabulary description and documentation
###

<> a owl:Ontology;
  foaf:maker <http://sebastian.tramp.name>;
  doap:maintainer <http://sebastian.tramp.name>;
  doap:homepage <https://github.com/AKSW/site.ontowiki>;
  vann:preferredNamespacePrefix "site";
  vann:preferredNamespaceUri "http://ns.ontowiki.net/SysOnt/Site/";
  vann:changes <https://github.com/AKSW/site.ontowiki/commits/master/schema/schema.ttl>;
  rdfs:label "OntoWiki site extension domain vocabulary";
  rdfs:isDefinedBy <http://ns.ontowiki.net/SysOnt/Site/> .

<http://sebastian.tramp.name> a foaf:Person; foaf:name "Sebastian Tramp".
